some progress

src/SSA.v
@@ -1,7 +1,7 @@
 From Coq Require Import List ZArith FSets OrderedType.
 From mathcomp Require Import ssreflect ssrnat ssrbool eqtype seq ssrfun.
 From nbits Require Import NBits.
-From BitBlasting Require Import Typ TypEnv State.
+From BitBlasting Require Import Typ TypEnv State BBCommon.
 From ssrlib Require Import Var SsrOrder FMaps ZAriths Tactics Lists FSets.
 From Cryptoline Require Import DSL.
 
@@ -336,8 +336,10 @@ Section MakeSSA.
   (* TODO: check defintion *)
   (* map only keys *)
 
+  Definition add_to_ste m k v (e: SSATE.env) := SSATE.add (ssa_var m k) v e.
+
   Definition ssa_typenv (m: vmap) (te: TE.env) : SSATE.env :=
-    TE.fold (fun k v e => SSATE.add (ssa_var m k) v e) te (SSATE.empty typ).
+    TE.fold (add_to_ste m) te (SSATE.empty typ).
 
   (* TODO: Define SSA translation *)
   Definition ssa_spec (s : DSL.spec) : SSA.spec :=
@@ -1442,34 +1444,26 @@ Section MakeSSA.
                  (SSAVS.union (ssa_vars m1 vs) (SSA.vars_instr si)).
   Proof.
     case: i =>  /=; intros;
-                  (match goal with
-                   | H : (_, _) = (_, _) |- _ => case: H => <- <- /=
-                   end
-                  );
-                  try first [
-                        exact: ssa_vars_instr_subset_1lv |
-                        exact: ssa_vars_instr_subset11 |
-                        exact: ssa_vars_instr_subset12 |
-                        exact: ssa_vars_instr_subset13 |
-                        exact: ssa_vars_instr_subset21 |
-                        exact: ssa_vars_instr_subset22 |
-                        exact: ssa_vars_instr_subset23 |
-                        exact: ssa_vars_instr_subset_1lv_3ra |
-                        exact: ssa_vars_instr_subset_2lv_3ra
-                      ].
+                 (match goal with
+                  | H : (_, _) = (_, _) |- _ => case: H => <- <- /=
+                  end
+                 );
+                 try first [
+                       exact: ssa_vars_instr_subset_1lv |
+                       exact: ssa_vars_instr_subset11 |
+                       exact: ssa_vars_instr_subset12 |
+                       exact: ssa_vars_instr_subset13 |
+                       exact: ssa_vars_instr_subset21 |
+                       exact: ssa_vars_instr_subset22 |
+                       exact: ssa_vars_instr_subset23 |
+                       exact: ssa_vars_instr_subset_1lv_3ra |
+                       exact: ssa_vars_instr_subset_2lv_3ra
+                     ].
     - (* Inop *)
       rewrite ssa_vars_union ssa_vars_empty.
       exact: SSAVS.Lemmas.subset_refl.
     - rewrite ssa_vars_union. rewrite ssa_vars_bexp_comm.
       exact: SSAVS.Lemmas.subset_refl.
-  (*
-    - rewrite ssa_vars_union. rewrite ssa_vars_bexp_comm.
-      exact: SSAVS.Lemmas.subset_refl.
-    - rewrite ssa_vars_union. rewrite ssa_vars_ebexp_comm.
-      exact: SSAVS.Lemmas.subset_refl.
-    - rewrite ssa_vars_union. rewrite ssa_vars_rbexp_comm.
-      exact: SSAVS.Lemmas.subset_refl.
-   *)
   Qed.
 
   Lemma ssa_vars_post_subset vs m1 m2 p sp g :
@@ -1504,12 +1498,36 @@ Section MakeSSA.
   Definition state_equiv (m : vmap) (s :Store.t) (ss : SSAStore.t) : Prop :=
     forall x, Store.acc x s = SSAStore.acc (x, get_index x m) ss.
 
+  (** Convert a DSL state to an SSA state. *)
 
-  Lemma ssa_typenv_preserve m TE v:
-    SSATE.vtyp (ssa_var m v) (ssa_typenv m TE) = TE.vtyp v TE.
-    (* correct bc. ssa_var is injective *)
-    (* TODO: need some works *)
-  Admitted.
+  Definition ssa_state (m : vmap) (s : Store.t) : SSAStore.t :=
+    fun v =>
+      if (sidx v) == get_index (svar v) m
+      then Store.acc (svar v) s
+      else Store.acc (svar v) Store.empty.
+
+  Lemma acc_ssa_state_eq m s v i:
+    i == get_index v m ->
+    SSAStore.acc (v, i) (ssa_state m s) = Store.acc v s.
+  Proof.
+    move=> Heq.
+    rewrite /ssa_state /SSAStore.acc /SSAStore.S.acc /=.
+    rewrite (eqP Heq) eqxx.
+    reflexivity.
+  Qed.
+
+  Lemma ssa_state_equiv m s:
+    state_equiv m s (ssa_state m s).
+  Proof.
+    move=> x.
+    rewrite (acc_ssa_state_eq _ (eqxx (get_index x m))).
+    reflexivity.
+  Qed.
+
+  (* Type Environment Equivalence *)
+
+  Definition typenv_equiv (m : vmap) (te : TE.env) (ste : SSATE.env) : Prop :=
+    forall x, TE.vtyp x te = SSATE.vtyp (x, get_index x m) ste.
 
   Lemma pair_neq1 :
     forall (T : eqType) (a b c d : T),
@@ -1531,6 +1549,176 @@ Section MakeSSA.
     case: H => Hac Hbd.
     apply/idP: Hne.
     rewrite Hbd; exact: eqxx.
+  Qed.
+
+  Lemma ssa_typenv_equiv_add (m: vmap) (te: TE.env) (ste: SSATE.env) x typ:
+    typenv_equiv m te ste ->
+    typenv_equiv m (TE.add x typ te) (SSATE.add (ssa_var m x) typ ste).
+  Proof.
+    move=> H.
+    intros y.
+    case Heq: (y==x).
+    - move/idP: Heq => Heq.
+      rewrite (TE.vtyp_add_eq Heq).
+      rewrite -/(ssa_var m y).
+      have Hseq: (ssa_var m y) == (ssa_var m x) by rewrite (eqP Heq).
+      rewrite (SSATE.vtyp_add_eq Hseq).
+      reflexivity.
+    - move/idP/negP: Heq => Hneq.
+      rewrite (TE.vtyp_add_neq Hneq).
+      rewrite -/(ssa_var m y).
+      have Hsneq: (ssa_var m y) != (ssa_var m x).
+      {
+        rewrite /ssa_var.
+        exact: (pair_neq1 _ _ Hneq).
+      }
+      rewrite (SSATE.vtyp_add_neq Hsneq).
+      exact: H.
+  Qed.
+
+  Lemma typenv_equiv_empty (m: vmap):
+    typenv_equiv m (TE.empty typ) (SSATE.empty typ).
+  Proof.
+    intros x.
+    have Hnmem: (~~ TE.mem x (TE.empty typ)) by rewrite TE.Lemmas.empty_a.
+    have Hsnmem: (~~ SSATE.mem (ssa_var m x) (SSATE.empty typ)) by rewrite SSATE.Lemmas.empty_a.
+    rewrite (TE.not_mem_vtyp Hnmem).
+    rewrite (SSATE.not_mem_vtyp Hsnmem).
+    reflexivity.
+  Qed.
+
+  Lemma ssa_typenv_equiv_empty (m: vmap) (te: TE.env):
+    TE.Empty te ->
+    typenv_equiv m te (ssa_typenv m te).
+  Proof.
+    move=> Hempty.
+    move: m.
+    (* intros x. *)
+    rewrite /ssa_typenv /=.
+    move=> m.
+    have Heq: (TE.fold (add_to_ste m) te (SSATE.empty typ)) = (SSATE.empty typ).
+    {
+
+      apply (DSL.TEKS.MLemmas.OP.P.fold_Empty _ (add_to_ste m) (SSATE.empty typ) Hempty).
+    }
+    rewrite Heq.
+    intros x.
+    move: (DSL.TEKS.MLemmas.Empty_mem x Hempty) => Hnm.
+    rewrite (TE.not_mem_vtyp Hnm).
+    have Hsnmem: (~~ SSATE.mem (ssa_var m x) (SSATE.empty typ)) by rewrite SSATE.Lemmas.empty_a.
+    rewrite (SSATE.not_mem_vtyp Hsnmem).
+    reflexivity.
+  Qed.
+
+  Instance add_to_set_proper m:
+    Proper (TE.SE.eq ==> eq ==> SSATE.Equal ==> SSATE.Equal) (add_to_ste m).
+  Proof.
+    move=> x y Hxy a b -> s1 s2 Heq.
+    rewrite /add_to_ste.
+    rewrite Heq.
+    rewrite (eqP Hxy).
+    reflexivity.
+  Qed.
+
+  Lemma add_to_set_transpose_neqkey m:
+    DSL.TEKS.MLemmas.OP.P.transpose_neqkey SSATE.Equal (add_to_ste m).
+  Proof.
+    move=> x y a b s Hxy.
+    rewrite /add_to_ste.
+    rewrite /SSATE.Equal.
+    move=> z.
+    have Hnxy: (ssa_var m x) != (ssa_var m y).
+    {
+      rewrite pair_neq1.
+      done.
+        by move/idP: Hxy.
+    }
+    case H1: (z == ssa_var m x); case H2: (z == ssa_var m y).
+    - move/idP/eqP: H1 => H1. move/idP/eqP: H2 => H2.
+      rewrite -H1 -H2 in Hnxy.
+      move/eqP: Hnxy => Hnxy.
+        by destruct Hnxy.
+    - move/idP: H1 => H1. move/negP: H2 => H2.
+      rewrite (SSA.TEKS.MLemmas.find_add_eq H1).
+      rewrite (SSA.TEKS.MLemmas.find_add_neq H2).
+      rewrite (SSA.TEKS.MLemmas.find_add_eq H1).
+      reflexivity.
+    - move/idP: H2 => H2. move/negP: H1 => H1.
+      rewrite (SSA.TEKS.MLemmas.find_add_eq H2).
+      rewrite (SSA.TEKS.MLemmas.find_add_neq H1).
+      rewrite (SSA.TEKS.MLemmas.find_add_eq H2).
+      reflexivity.
+    - move/negP: H1 => H1. move/negP: H2 => H2.
+      rewrite (SSA.TEKS.MLemmas.find_add_neq H1).
+      rewrite (SSA.TEKS.MLemmas.find_add_neq H2).
+      rewrite (SSA.TEKS.MLemmas.find_add_neq H2).
+      rewrite (SSA.TEKS.MLemmas.find_add_neq H1).
+      reflexivity.
+  Qed.
+
+  Lemma ssa_typenv_equiv (m: vmap) (te: TE.t typ):
+    typenv_equiv m te (ssa_typenv m te).
+  Proof.
+    move: te.
+    apply DSL.TEKS.MLemmas.OP.P.map_induction.
+    intros te.
+    - exact: ssa_typenv_equiv_empty.
+    - intros te te' IH x e HnIn HAdd y.
+      rewrite /ssa_typenv.
+      move: (DSL.TEKS.MLemmas.Add_mem_add x HAdd) => Hmem.
+      move: (DSL.TEKS.MLemmas.Add_in HAdd) => Hin.
+      rewrite /TE.vtyp.
+      replace (TE.vtyp y te') with
+          (
+            match VM.find y te' with
+            | None => TE.deftyp
+            | Some ty => ty
+            end
+
+          ) by reflexivity.
+      rewrite -/(ssa_var m y).
+      replace (SSATE.vtyp (ssa_var m y) (TE.fold (add_to_ste m) te' (SSATE.empty typ))) with
+          (
+            match SSAVM.find (ssa_var m y) (TE.fold (add_to_ste m) te' (SSATE.empty typ)) with
+            | None => SSATE.deftyp
+            | Some ty => ty
+            end
+
+          ) by reflexivity.
+      move: (DSL.TEKS.MLemmas.OP.P.fold_Add
+               (SSA.TEKS.MLemmas.F.Equal_ST typ)
+               (add_to_set_proper m)
+               (add_to_set_transpose_neqkey m)
+               (SSATE.empty typ)
+               HnIn HAdd) => Heq.
+      rewrite -/(ssa_var m y).
+      rewrite /SSATE.Equal in Heq.
+      rewrite (Heq (ssa_var m y)).
+      case Hyx: (y == x).
+      + rewrite (eqP Hyx).
+        rewrite HAdd.
+        rewrite (DSL.TEKS.MLemmas.find_add_eq).
+        rewrite /add_to_ste.
+        rewrite SSA.TEKS.MLemmas.find_add_eq.
+        reflexivity.
+        reflexivity.
+        reflexivity.
+      + rewrite HAdd.
+        move/negP: Hyx => Hyx.
+        rewrite (DSL.TEKS.MLemmas.find_add_neq Hyx).
+        rewrite /add_to_ste.
+        rewrite SSA.TEKS.MLemmas.find_add_neq.
+        exact: IH.
+        move/idP: Hyx => Hyx.
+        rewrite /SSATE.SE.eq.
+        rewrite /ssa_var.
+        apply /negP.
+        exact: (pair_neq1 _ _ Hyx).
+  Qed.
+
+  Corollary ssa_typenv_preserve m TE v:
+    TE.vtyp v TE= SSATE.vtyp (ssa_var m v) (ssa_typenv m TE) .
+    exact: ssa_typenv_equiv.
   Qed.
 
   Lemma ssa_eval_eunop :
@@ -1579,13 +1767,14 @@ Section MakeSSA.
     - reflexivity.
   Qed.
 
-  Lemma ssa_eval_eexp m TE s ss (e : DSL.eexp) :
+  Lemma ssa_eval_eexp m s ss te ste (e : DSL.eexp) :
     state_equiv m s ss ->
-    SSA.eval_eexp (ssa_eexp m e) (ssa_typenv m TE) ss = DSL.eval_eexp e TE s.
+    typenv_equiv m te ste ->
+    SSA.eval_eexp (ssa_eexp m e) ste ss = DSL.eval_eexp e te s.
   Proof.
-    move=> Heq; elim: e => /=.
-    - move=> v. rewrite (Heq v).
-      rewrite ssa_typenv_preserve.
+    move=> Hseq Hteq; elim: e => /=.
+    - move=> v. rewrite (Hseq v).
+      rewrite Hteq.
       reflexivity.
     - reflexivity.
     - move=> op e IH. rewrite IH. reflexivity.
@@ -1605,32 +1794,35 @@ Section MakeSSA.
     - move=> w e IH p. rewrite IH. reflexivity.
   Qed.
 
-  Lemma ssa_eval_ebexp m TE s ss e :
+  Lemma ssa_eval_ebexp m s ss te ste e :
     state_equiv m s ss ->
-    SSA.eval_ebexp (ssa_ebexp m e) (ssa_typenv m TE) ss <-> DSL.eval_ebexp e TE s.
+    typenv_equiv m te ste ->
+    SSA.eval_ebexp (ssa_ebexp m e) ste ss <-> DSL.eval_ebexp e te s.
   Proof.
-    move=> Heq; elim: e => /=.
+    move=> Hseq Hteq; elim: e => /=.
     - done.
-    - move=> e1 e2. rewrite 2!(ssa_eval_eexp _ _ Heq). done.
-    - move=> e1 e2 p. rewrite 3!(ssa_eval_eexp _ _ Heq). done.
+    - move=> e1 e2. rewrite 2!(ssa_eval_eexp _ Hseq Hteq). done.
+    - move=> e1 e2 p. rewrite 3!(ssa_eval_eexp _ Hseq Hteq). done.
     - move=> e1 [IH11 IH12] e2 [IH21 IH22]. tauto.
   Qed.
 
-  Lemma ssa_eval_ebexp1 m TE s ss e :
+  Lemma ssa_eval_ebexp1 m s ss te ste e :
     state_equiv m s ss ->
-    SSA.eval_ebexp (ssa_ebexp m e) (ssa_typenv m TE) ss -> DSL.eval_ebexp e TE s.
+    typenv_equiv m te ste ->
+    SSA.eval_ebexp (ssa_ebexp m e) ste ss -> DSL.eval_ebexp e te s.
   Proof.
-    move=> Heq He.
-    move: (ssa_eval_ebexp TE e Heq) => [H1 H2].
+    move=> Hseq Hteq He.
+    move: (ssa_eval_ebexp e Hseq Hteq) => [H1 H2].
     exact: (H1 He).
   Qed.
 
-  Lemma ssa_eval_ebexp2 m TE s ss e :
+  Lemma ssa_eval_ebexp2 m s ss te ste e :
     state_equiv m s ss ->
-    DSL.eval_ebexp e TE s -> SSA.eval_ebexp (ssa_ebexp m e) (ssa_typenv m TE) ss.
+    typenv_equiv m te ste ->
+    DSL.eval_ebexp e te s -> SSA.eval_ebexp (ssa_ebexp m e) ste ss.
   Proof.
-    move=> Heq He.
-    move: (ssa_eval_ebexp TE e Heq) => [H1 H2].
+    move=> Hseq Hteq He.
+    move: (ssa_eval_ebexp e Hseq Hteq) => [H1 H2].
     exact: (H2 He).
   Qed.
 
@@ -1665,30 +1857,33 @@ Section MakeSSA.
     exact: (H2 He).
   Qed.
 
-  Lemma ssa_eval_bexp m TE s ss e :
+  Lemma ssa_eval_bexp m s ss te ste e :
     state_equiv m s ss ->
-    SSA.eval_bexp (ssa_bexp m e) (ssa_typenv m TE) ss <-> DSL.eval_bexp e TE s.
+    typenv_equiv m te ste ->
+    SSA.eval_bexp (ssa_bexp m e) ste ss <-> DSL.eval_bexp e te s.
   Proof.
-    move=> Heq. split; move=> [H1 H2].
-    - exact: (conj (ssa_eval_ebexp1 Heq H1) (ssa_eval_rbexp1 Heq H2)).
-    - exact: (conj (ssa_eval_ebexp2 Heq H1) (ssa_eval_rbexp2 Heq H2)).
+    move=> Hseq Hteq. split; move=> [H1 H2].
+    - exact: (conj (ssa_eval_ebexp1 Hseq Hteq H1) (ssa_eval_rbexp1 Hseq H2)).
+    - exact: (conj (ssa_eval_ebexp2 Hseq Hteq H1) (ssa_eval_rbexp2 Hseq H2)).
   Qed.
 
-  Lemma ssa_eval_bexp1 m TE s ss e :
+  Lemma ssa_eval_bexp1 m s ss te ste e :
     state_equiv m s ss ->
-    SSA.eval_bexp (ssa_bexp m e) (ssa_typenv m TE ) ss -> DSL.eval_bexp e TE s.
+    typenv_equiv m te ste ->
+    SSA.eval_bexp (ssa_bexp m e) ste ss -> DSL.eval_bexp e te s.
   Proof.
-    move=> Heq He.
-    move: (ssa_eval_bexp TE e Heq) => [H1 H2].
+    move=> Hseq Hteq He.
+    move: (ssa_eval_bexp e Hseq Hteq) => [H1 H2].
     exact: (H1 He).
   Qed.
 
-  Lemma ssa_eval_bexp2 m s TE ss e :
+  Lemma ssa_eval_bexp2 m s ss te ste e :
     state_equiv m s ss ->
-    DSL.eval_bexp e TE s -> SSA.eval_bexp (ssa_bexp m e) (ssa_typenv m TE) ss.
+    typenv_equiv m te ste ->
+    DSL.eval_bexp e te s -> SSA.eval_bexp (ssa_bexp m e) ste ss.
   Proof.
-    move=> Heq He.
-    move: (ssa_eval_bexp TE e Heq) => [H1 H2].
+    move=> Hseq Hteq He.
+    move: (ssa_eval_bexp e Hseq Hteq) => [H1 H2].
     exact: (H2 He).
   Qed.
 
@@ -1706,6 +1901,24 @@ Section MakeSSA.
     - move/idP/negP: Hyx => Hyx.
       rewrite (Store.acc_upd_neq Hyx).
       rewrite (SSAStore.acc_upd_neq (pair_neq1 _ _ Hyx)).
+      rewrite (get_upd_index_neq _ Hyx).
+      exact: Heq.
+  Qed.
+
+  Lemma state_equiv_Upd m s1 s2 ss1 ss2 x v :
+    state_equiv m s1 ss1 ->
+    Store.Upd x v s1 s2 ->
+    SSAStore.Upd (ssa_var (upd_index x m) x) v ss1 ss2 ->
+    state_equiv (upd_index x m) s2 ss2.
+  Proof.
+    move=> Heq Hupd Hsupd y.
+    case Hyx: (y == x) => /=.
+    - rewrite (Store.acc_Upd_eq Hyx Hupd).
+      rewrite (eqP Hyx) (SSAStore.acc_Upd_eq (eqxx (ssa_var _ x)) Hsupd).
+      reflexivity.
+    - move/idP/negP: Hyx => Hyx.
+      rewrite (Store.acc_Upd_neq Hyx Hupd).
+      rewrite (SSAStore.acc_Upd_neq (pair_neq1 _ _ Hyx) Hsupd).
       rewrite (get_upd_index_neq _ Hyx).
       exact: Heq.
   Qed.
@@ -1731,244 +1944,394 @@ Section MakeSSA.
       exact: state_equiv_upd.
   Qed.
 
-  (* Ltac ssa_eval_state_equiv_tac := *)
-  (*   simpl; intros; *)
-  (*   let rec tac := *)
-  (*       lazymatch goal with *)
-  (*       | H : (_, _) = (_, _) |- _ => *)
-  (*         case: H; intros; subst; simpl; tac *)
-  (*       | H : state_equiv ?m ?s ?ss *)
-  (*         |- context f [SSA.eval_atomic (ssa_atomic ?m ?a) ?ss] => *)
-  (*         rewrite (ssa_eval_atomic a H); tac *)
-  (*       | H : state_equiv ?m ?s ?ss *)
-  (*         |- context f [SSAStore.acc (ssa_var ?m ?a) ?ss] => *)
-  (*         rewrite -(H a); tac *)
-  (*       | H : state_equiv ?m ?s ?ss |- _ => *)
-  (*         try first [ exact: (state_equiv_upd _ _ H) | *)
-  (*                     exact: (state_equiv_upd2 _ _ _ _ H) ] *)
-  (*       end in *)
-  (*   tac. *)
+  Lemma state_equiv_Upd2 m s1 s2 ss1 ss2 x vx y vy :
+    state_equiv m s1 ss1 ->
+    Store.Upd2 x vx y vy s1 s2 ->
+    SSAStore.Upd2 (ssa_var (upd_index x m) x) vx
+                  (ssa_var (upd_index y (upd_index x m)) y) vy
+                  ss1 ss2 ->
+    state_equiv (upd_index y (upd_index x m)) s2 ss2.
+  Proof.
+    move=> Heq Hupd Hsupd z.
+    case Hzy: (z == y) => /=.
+    - rewrite (Store.acc_Upd_eq Hzy Hupd).
+      rewrite (eqP Hzy) (SSAStore.acc_Upd_eq (eqxx (ssa_var _ y)) Hsupd).
+      reflexivity.
+    - move/idP/negP: Hzy => Hzy.
+      rewrite (Store.acc_Upd_neq Hzy Hupd).
+      rewrite (SSAStore.acc_Upd_neq (pair_neq1 _ _ Hzy) Hsupd).
+      rewrite (get_upd_index_neq _ Hzy).
+      exact: state_equiv_Upd.
+  Qed.
 
-  (* Lemma ssa_eval_instr : *)
-  (*   forall m1 m2 TE1 TE2 s1 s2 ss1 ss2 i si, *)
-  (*     ssa_instr m1 i = (m2, si) -> *)
-  (*     ssa_typenv m1 TE1 = TE2 -> *)
-  (*     state_equiv m1 s1 ss1 -> *)
-  (*     DSL.eval_instr TE1 i = s2 -> *)
-  (*     SSA.eval_instr TE2 ss1 si = ss2 -> *)
-  (*     state_equiv m2 s2 ss2. *)
-  (* Proof. *)
-  (*   move=> m1 m2 s1 s2 ss1 ss2 i. *)
-  (*   case: i; by ssa_eval_state_equiv_tac. *)
-  (* Qed. *)
+  Lemma typenv_equiv_add m te ste x typ :
+    typenv_equiv m te ste ->
+    typenv_equiv (upd_index x m)
+                 (TE.add x typ te)
+                 (SSATE.add (ssa_var (upd_index x m) x) typ ste).
+  Proof.
+    move=> Heq y.
+    case Hyx: (y == x) => /=.
+    - rewrite (TE.vtyp_add_eq Hyx).
+      rewrite (eqP Hyx) (SSATE.vtyp_add_eq (eqxx (ssa_var _ x))).
+      reflexivity.
+    - move/idP/negP: Hyx => Hyx.
+      rewrite (TE.vtyp_add_neq Hyx).
+      rewrite (SSATE.vtyp_add_neq (pair_neq1 _ _ Hyx)).
+      rewrite (get_upd_index_neq _ Hyx).
+      exact: Heq.
+  Qed.
 
-  (*
-  (* TODO: Check if all variables in a program are not indexed. *)
+  Lemma typenv_equiv_add2 m te ste x xtyp y ytyp:
+    typenv_equiv m te ste ->
+    typenv_equiv (upd_index y (upd_index x m))
+                 (TE.add y ytyp (TE.add x xtyp te))
+                 (SSATE.add (ssa_var (upd_index y (upd_index x m)) y) ytyp
+                            (SSATE.add (ssa_var (upd_index x m) x) xtyp ste)).
+  Proof.
+    move=> Heq z.
+    case Hzy: (z == y) => /=.
+    - rewrite (TE.vtyp_add_eq Hzy).
+      rewrite (eqP Hzy) (SSATE.vtyp_add_eq (eqxx (ssa_var _ y))).
+      reflexivity.
+    - move/idP/negP: Hzy => Hzy.
+      rewrite (TE.vtyp_add_neq Hzy).
+      rewrite (SSATE.vtyp_add_neq (pair_neq1 _ _ Hzy)).
+      rewrite (get_upd_index_neq _ Hzy).
+      exact: typenv_equiv_add.
+  Qed.
 
-  Definition unindexed_var (v : var) : bool :=
-    vidx v == 1.
+  Hint Resolve typenv_equiv_add typenv_equiv_add2.
 
-  Definition unindexed_vars vs := VS.for_all unindexed_var vs.
+  Lemma ssa_atyp m a te ste:
+    typenv_equiv m te ste ->
+    SSA.atyp (ssa_atomic m a) ste = DSL.atyp a te.
+  Proof.
+    elim: a m te ste => /=; intros.
+    - by rewrite H.
+    - done.
+  Qed.
 
-  Definition unindexed_atomic  (a : atomic) : bool :=
-    match a with
-    | Avar v => unindexed_var v
-    | Aconst ty n => true
+  Ltac ssa_eval_instr_succ_tac :=
+    match goal with
+    | H: ssa_instr _ _ = (?p1, ?p2) |- _ =>
+      case: H => <- <-
+    | |- _ /\ _ => split
+    | |- exists ss2 , _ => eexists
+    | H: ?e |- ?e => exact: H
+    | |- context [SSA.instr_succ_typenv _ _] => rewrite /=
+    | Heq: state_equiv ?m ?s ?ss |- context [SSA.eval_atomic (ssa_atomic ?m ?a) ?ss]
+      => rewrite (ssa_eval_atomic a Heq)
+    | Heq: typenv_equiv ?m1 ?te1 ?ste1 |- context[SSA.atyp (ssa_atomic ?m1 ?a) ?ste1]
+      => rewrite (ssa_atyp a Heq)
+    | |- SSA.eval_instr _ _ _ _ => econstructor
+    | |- SSAStore.Upd ?x ?v ?s ?s => exact: SSAStore.Upd_upd
+    | |- SSAStore.Upd ?x ?v ?s1 ?s2 => exact: SSAStore.Upd_upd
+    | |- SSAStore.Upd2 ?x1 ?v1 ?x2 ?v2 ?s1 ?s2 => exact: SSAStore.Upd2_upd2
+    | H: DSL.instr_succ_typenv _ ?te1 = ?te2 |- context [?te2]
+      => rewrite /= in H; erewrite <- H; clear H
+    | |- state_equiv _ _ (SSAStore.upd ?x ?v ?s) => eapply state_equiv_Upd
+    | |- state_equiv _ _ (SSAStore.upd2 ?x1 ?v1 ?x2 ?v2 ?s) => eapply state_equiv_Upd2
+    | H : state_equiv ?m _ _ |- state_equiv ?m _ _ => exact: H
+    | H: typenv_equiv ?m1 ?te1 ?ste1
+      |- typenv_equiv (upd_index ?t ?m1) (TE.add ?t ?typ ?te1) ?ste2
+      => eapply typenv_equiv_add
+    | H: typenv_equiv ?m1 ?te1 ?ste1
+      |- typenv_equiv (upd_index ?t2 (upd_index ?t ?m1)) (TE.add ?t2 ?typ2 (TE.add ?t ?typ ?te1)) ?ste2
+      => eapply typenv_equiv_add2
+    | H: DSL.eval_instr _ _ _ _ |- _ => inversion H; subst; clear H
+    | |- ?e => progress (eauto)
+    | |- ?e => fail "not match" e
     end.
 
-  Fixpoint unindexed_eexp (e: eexp) :=
-    match e with
-    | Evar v => unindexed_var v
-    | Econst c => true
-    | Eunop op e => unindexed_eexp e
-    | Ebinop op e1 e2 => unindexed_eexp e1 && unindexed_eexp e2
-    end.
+  Lemma ssa_eval_instr_succ m1 m2 s1 s2 te1 te2 ste1 ss1 i si:
+    ssa_instr m1 i = (m2, si) ->
+    state_equiv m1 s1 ss1 ->
+    typenv_equiv m1 te1 ste1 ->
+    DSL.eval_instr te1 i s1 s2 ->
+    DSL.instr_succ_typenv i te1 = te2 ->
+    exists ss2 ste2,
+      SSA.eval_instr ste1 si ss1 ss2 /\
+      SSA.instr_succ_typenv si ste1 = ste2 /\
+      state_equiv m2 s2 ss2 /\
+      typenv_equiv m2 te2 ste2.
+  Proof.
+    elim: i m1 m2 s1 s2 te1 te2 ste1 ss1 si; intros.
+    - repeat ssa_eval_instr_succ_tac.
+    - repeat ssa_eval_instr_succ_tac.
+    - repeat ssa_eval_instr_succ_tac.
+    - ssa_eval_instr_succ_tac.
+      inversion_clear H2.
+      exists (SSAStore.upd (ssa_var (upd_index t m1) t) n ss1).
+      repeat ssa_eval_instr_succ_tac.
+    - ssa_eval_instr_succ_tac.
+      inversion_clear H2.
+      + (* cmovT *)
+        repeat ssa_eval_instr_succ_tac.
+      + (* cmovF *)
+        ssa_eval_instr_succ_tac.
+        ssa_eval_instr_succ_tac.
+        ssa_eval_instr_succ_tac.
+        apply SSA.EIcmovF; repeat ssa_eval_instr_succ_tac.
+        repeat ssa_eval_instr_succ_tac.
+    - repeat ssa_eval_instr_succ_tac.
+    - repeat ssa_eval_instr_succ_tac.
+    - repeat ssa_eval_instr_succ_tac.
+    - repeat ssa_eval_instr_succ_tac.
+    - repeat ssa_eval_instr_succ_tac.
+    - repeat ssa_eval_instr_succ_tac.
+    - repeat ssa_eval_instr_succ_tac.
+    - repeat ssa_eval_instr_succ_tac.
+    - repeat ssa_eval_instr_succ_tac.
+    - repeat ssa_eval_instr_succ_tac.
+    - repeat ssa_eval_instr_succ_tac.
+    - repeat ssa_eval_instr_succ_tac.
+    - repeat ssa_eval_instr_succ_tac.
+    - repeat ssa_eval_instr_succ_tac.
+    - repeat ssa_eval_instr_succ_tac.
+    - repeat ssa_eval_instr_succ_tac.
+    - ssa_eval_instr_succ_tac.
+      rewrite /= in H3.
+      inversion H2; subst;clear H2.
+      + ssa_eval_instr_succ_tac.
+        ssa_eval_instr_succ_tac.
+        ssa_eval_instr_succ_tac.
+        eapply SSA.EIsplitU.
+        repeat ssa_eval_instr_succ_tac.
+        repeat ssa_eval_instr_succ_tac.
+        repeat ssa_eval_instr_succ_tac.
+      + ssa_eval_instr_succ_tac.
+        ssa_eval_instr_succ_tac.
+        ssa_eval_instr_succ_tac.
+        eapply SSA.EIsplitS.
+        repeat ssa_eval_instr_succ_tac.
+        repeat ssa_eval_instr_succ_tac.
+        repeat ssa_eval_instr_succ_tac.
+    - repeat ssa_eval_instr_succ_tac.
+    - repeat ssa_eval_instr_succ_tac.
+    - repeat ssa_eval_instr_succ_tac.
+    - ssa_eval_instr_succ_tac.
+      inversion H2; subst; clear H2.
+      ssa_eval_instr_succ_tac.
+      ssa_eval_instr_succ_tac.
+      ssa_eval_instr_succ_tac.
+      ssa_eval_instr_succ_tac.
+      ssa_eval_instr_succ_tac.
+      ssa_eval_instr_succ_tac.
+      ssa_eval_instr_succ_tac.
+      ssa_eval_instr_succ_tac.
+      ssa_eval_instr_succ_tac.
+      ssa_eval_instr_succ_tac.
+      rewrite ssa_var_upd_eq.
+      (* rewrite (ssa_atyp a H1). *)
+      (* exact: SSAStore.Upd_upd. *)
+      (* rewrite /=. *)
+      repeat ssa_eval_instr_succ_tac.
+      rewrite /=.
+      repeat ssa_eval_instr_succ_tac.
+    - ssa_eval_instr_succ_tac.
+      inversion H2; subst; clear H2.
+      ssa_eval_instr_succ_tac.
+      ssa_eval_instr_succ_tac.
+      ssa_eval_instr_succ_tac.
+      ssa_eval_instr_succ_tac.
+      ssa_eval_instr_succ_tac.
+      ssa_eval_instr_succ_tac.
+      ssa_eval_instr_succ_tac.
+      ssa_eval_instr_succ_tac.
+      ssa_eval_instr_succ_tac.
+      ssa_eval_instr_succ_tac.
+      rewrite ssa_var_upd_eq.
+      rewrite /=.
+      repeat ssa_eval_instr_succ_tac.
+    - repeat ssa_eval_instr_succ_tac.
+    - ssa_eval_instr_succ_tac.
+      inversion H2; subst; clear H2.
+      ssa_eval_instr_succ_tac.
+      ssa_eval_instr_succ_tac.
+      ssa_eval_instr_succ_tac.
+      ssa_eval_instr_succ_tac.
+      erewrite (ssa_eval_bexp).
+      all: repeat ssa_eval_instr_succ_tac.
+  Qed.
 
-  Fixpoint unindexed_rexp (e: rexp) :=
-    match e with
-    | Rvar v => unindexed_var v
-    | Rconst w n => true
-    | Runop w op e => unindexed_rexp e
-    | Rbinop w op e1 e2 => unindexed_rexp e1 && unindexed_rexp e2
-    | Ruext w e i => unindexed_rexp e
-    | Rsext w e i => unindexed_rexp e
-    end.
+  Lemma ssa_eval_program_succ m1 m2 s1 s2 te1 te2 p sp ss1 ste1:
+    ssa_program m1 p = (m2, sp) ->
+    state_equiv m1 s1 ss1 ->
+    typenv_equiv m1 te1 ste1 ->
+    DSL.eval_program te1 p s1 s2 ->
+    DSL.program_succ_typenv p te1 = te2 ->
+    exists ss2 ste2,
+      SSA.eval_program ste1 sp ss1 ss2 /\
+      SSA.program_succ_typenv sp ste1 = ste2 /\
+      state_equiv m2 s2 ss2 /\
+      typenv_equiv m2 te2 ste2.
+  Proof.
+    elim: p m1 m2 s1 s2 te1 te2 sp ss1 ste1.
+    - move=> m1 m2 s1 s2 te1 te2 sp ss1 ste1 /=.
+      case=> <- <-.
+      move=> Hse Hte Hep Hteq.
+      rewrite /DSL.eval_program in Hep.
+      rewrite /= in Hep.
+      inversion Hep; subst.
+      exists ss1, ste1. split_andb_goal.
+      + constructor.
+      + constructor.
+      + assumption.
+      + assumption.
+    - move=> hd tl IH m1 m2 s1 s2 te1 te2 [| shd stl] ss1 ste1.
+      + move=> Hsp. rewrite /= in Hsp. move: Hsp.
+        case Hsi_hd: (ssa_instr m1 hd) => [sm1 shd].
+        case Hsp_tl: (ssa_program sm1 tl) => [sm2 stl].
+        inversion 1.
+      + move=> Hsp Hseq Hteq Hep Hpst.
+        inversion Hsp.
+        move: H0.
+        case Hsi_hd: (ssa_instr m1 hd) => [sm1 sshd].
+        case Hsp_tl: (ssa_program sm1 tl) => [sm2 sstl].
+        move=> Hpair.
+        case: Hpair => <- <- <-.
+        move: Hpst.
+        inversion Hep; subst.
+        move=> Hpst.
+        rewrite /= in Hpst.
+        remember (DSL.instr_succ_typenv hd te1) as te3.
+        symmetry in Heqte3.
+        move: (ssa_eval_instr_succ Hsi_hd Hseq Hteq H1 Heqte3) => Htmp.
+        destruct Htmp as [ss3 [ste3 Hwit]].
+        inversion Hwit as [Hseval [Hsstyp [Hseq2 Hteq2]]].
+        move: (IH _ _ _ _ _ _ _ _ _ Hsp_tl Hseq2 Hteq2 H4 Hpst) => HIH.
+        destruct HIH as [ss2 [ste2 Hswit]].
+        inversion Hswit as [Hsep [Hstyp [Hseq3 Hteq3]]].
+        exists ss2, ste2.
+        split_andb_goal.
+        eapply SSA.Econs.
+        * exact: Hseval.
+        * rewrite Hsstyp.
+        * exact: Hsep.
+        * rewrite /=.
+          by rewrite Hsstyp.
+        * exact: Hseq3.
+        * exact: Hteq3.
+  Qed.
 
-  Fixpoint unindexed_ebexp (e: ebexp) :=
-    match e with
-    | Etrue => true
-    | Eeq e1 e2 => unindexed_eexp e1 && unindexed_eexp e2
-    | Eeqmod e1 e2 p => unindexed_eexp e1 && unindexed_eexp e2 && unindexed_eexp p
-    | Eand e1 e2 => unindexed_ebexp e1 && unindexed_ebexp e2
-    end.
+  Lemma dessa_eval_instr_succ m1 m2 s1 ss1 ss2 te1 ste1 ste2 i si:
+      ssa_instr m1 i = (m2, si) ->
+      state_equiv m1 s1 ss1 ->
+      typenv_equiv m1 te1 ste1 ->
+      SSA.eval_instr ste1 si ss1 ss2 ->
+      SSA.instr_succ_typenv si ste1 = ste2 ->
+      exists s2 te2,
+        DSL.eval_instr te1 i s1 s2 /\
+        DSL.instr_succ_typenv i te1 = te2 /\
+        state_equiv m2 s2 ss2 /\
+        typenv_equiv m2 te2 ste2.
+  Proof.
+  Admitted.
 
-  Fixpoint unindexed_rbexp (e: rbexp) :=
-    match e with
-    | Rtrue => true
-    | Req w e1 e2 => unindexed_rexp e1 && unindexed_rexp e2
-    | Rcmp w op e1 e2 => unindexed_rexp e1 && unindexed_rexp e2
-    | Rneg e =>  unindexed_rbexp e
-    | Rand e1 e2 => unindexed_rbexp e1 && unindexed_rbexp e2
-    | Ror e1 e2 => unindexed_rbexp e1 && unindexed_rbexp e2
-    end.
+  Lemma dessa_eval_program_succ m1 m2 s1 ss1 ss2 te1 ste1 ste2 p sp:
+    ssa_program m1 p = (m2, sp) ->
+    state_equiv m1 s1 ss1 ->
+    typenv_equiv m1 te1 ste1 ->
+    SSA.eval_program ste1 sp ss1 ss2 ->
+    SSA.program_succ_typenv sp ste1 = ste2 ->
+    exists s2 te2,
+      DSL.eval_program te1 p s1 s2 /\
+      DSL.program_succ_typenv p te1 = te2 /\
+      state_equiv m2 s2 ss2 /\
+      typenv_equiv m2 te2 ste2.
+  Proof.
+  Admitted.
 
-  Definition unindexed_bexp e := unindexed_ebexp (eqn_bexp e) && unindexed_rbexp (rng_bexp e).
+  (** Convert an SSA state to a DSL state. *)
 
-  Definition unindexed_instr (i: instr) : bool :=
-    match i with
-    | Imov v a
-    | Ishl v a _ =>
-      let v := unindexed_var v in
-      let a := unindexed_atomic a in
-      v && a
-    | Icshl vh vl a1 a2 _ =>
-      let vh := unindexed_var vh in
-      let vl := unindexed_var vl in
-      let a1 := unindexed_atomic a1 in
-      let a2 := unindexed_atomic a2 in
-      vh && vl && a1 && a2
-    | Inondet v =>
-      let v := unindexed_var v in v
-    | Icmov v c a1 a2 =>
-      let v := unindexed_var v in
-      let c := unindexed_atomic c in
-      let a1 := unindexed_atomic a1 in
-      let a2 := unindexed_atomic a2 in
-      v && c && a1 && a2
-    | Inop => true
-    | Inot v a =>
-      let v := unindexed_var v in
-      let a := unindexed_atomic a in
-      v && a
-    | Iadd v a1 a2 =>
-      let v := unindexed_var v in
-      let a1 := unindexed_atomic a1 in
-      let a2 := unindexed_atomic a2 in
-      v && a1 && a2
-    | Iadds c v a1 a2
-    | Iaddr c v a1 a2 =>
-      let c := unindexed_var c in
-      let v := unindexed_var v in
-      let a1 := unindexed_atomic a1 in
-      let a2 := unindexed_atomic a2 in
-      c && v && a1 && a2
-    | Iadc v a1 a2 y =>
-      let v := unindexed_var v in
-      let a1 := unindexed_atomic a1 in
-      let a2 := unindexed_atomic a2 in
-      let y := unindexed_atomic y in
-      v && a1 && a2 && y
-    | Iadcs c v a1 a2 y
-    | Iadcr c v a1 a2 y =>
-      let c := unindexed_var c in
-      let v := unindexed_var v in
-      let a1 := unindexed_atomic a1 in
-      let a2 := unindexed_atomic a2 in
-      let y := unindexed_atomic y in
-      c && v && a1 && a2 && y
-    | Isub v a1 a2 =>
-      let v := unindexed_var v in
-      let a1 := unindexed_atomic a1 in
-      let a2 := unindexed_atomic a2 in
-      v && a1 && a2
-    | Isubc c v a1 a2
-    | Isubb c v a1 a2
-    | Isubr c v a1 a2 =>
-      let c := unindexed_var c in
-      let v := unindexed_var v in
-      let a1 := unindexed_atomic a1 in
-      let a2 := unindexed_atomic a2 in
-      c && v && a1 && a2
-    | Isbc v a1 a2 y =>
-      let v := unindexed_var v in
-      let a1 := unindexed_atomic a1 in
-      let a2 := unindexed_atomic a2 in
-      let y := unindexed_atomic y in
-      v && a1 && a2 && y
-    | Isbcs c v a1 a2 y
-    | Isbcr c v a1 a2 y =>
-      let c := unindexed_var c in
-      let v := unindexed_var v in
-      let a1 := unindexed_atomic a1 in
-      let a2 := unindexed_atomic a2 in
-      let y := unindexed_atomic y in
-      c && v && a1 && a2 && y
-    | Isbb v a1 a2 y =>
-      let v := unindexed_var v in
-      let a1 := unindexed_atomic a1 in
-      let a2 := unindexed_atomic a2 in
-      let y := unindexed_atomic y in
-      v && a1 && a2 && y
-    | Isbbs c v a1 a2 y
-    | Isbbr c v a1 a2 y =>
-      let c := unindexed_var c in
-      let v := unindexed_var v in
-      let a1 := unindexed_atomic a1 in
-      let a2 := unindexed_atomic a2 in
-      let y := unindexed_atomic y in
-      c && v && a1 && a2 && y
-    | Imul v a1 a2 =>
-      let v := unindexed_var v in
-      let a1 := unindexed_atomic a1 in
-      let a2 := unindexed_atomic a2 in
-      v && a1 && a2
-    | Imuls c v a1 a2
-    | Imulr c v a1 a2 =>
-      let c := unindexed_var c in
-      let v := unindexed_var v in
-      let a1 := unindexed_atomic a1 in
-      let a2 := unindexed_atomic a2 in
-      c && v && a1 && a2
-    | Imull vh vl a1 a2 =>
-      let vh := unindexed_var vh in
-      let vl := unindexed_var vl in
-      let a1 := unindexed_atomic a1 in
-      let a2 := unindexed_atomic a2 in
-      vh && vl && a1 && a2
-    | Imulj v a1 a2 =>
-      let v := unindexed_var v in
-      let a1 := unindexed_atomic a1 in
-      let a2 := unindexed_atomic a2 in
-      v && a1 && a2
-    | Isplit vh vl a n =>
-      let vh := unindexed_var vh in
-      let vl := unindexed_var vl in
-      let a := unindexed_atomic a in
-      vh && vl && a
-    | Iand v a1 a2
-    | Ior v a1 a2
-    | Ixor v a1 a2 =>
-      let v := unindexed_var v in
-      let a1 := unindexed_atomic a1 in
-      let a2 := unindexed_atomic a2 in
-      v && a1 && a2
-    | Icast v a
-    | Ivpc v a =>
-      let v := unindexed_var v in
-      let a := unindexed_atomic a in
-      v && a
-    | Ijoin v ah al =>
-      let v := unindexed_var v in
-      let ah := unindexed_atomic ah in
-      let al := unindexed_atomic al in
-      v && ah && al
-    | Iassert e => unindexed_bexp e
-    | Iassume e => unindexed_bexp e
-    | Iecut e pwss => unindexed_ebexp e
-    | Ircut e pwss => unindexed_rbexp e
-    | Ighost vs e => unindexed_vars vs && unindexed_bexp e
-    end.
+  Definition dessa_state (m : vmap) (s : SSAStore.t) : Store.t :=
+    fun v => SSAStore.acc (v, get_index v m) s.
 
-  Fixpoint unindexed_program (p : program) : bool :=
-    match p with
-    | [::] => true
-    | hd::tl =>
-      let unidx_instr := unindexed_instr hd in
-      let unidx_tl := unindexed_program tl in
-      unidx_instr && unidx_tl
-    end.
+  Lemma acc_dessa_state :
+    forall (m : vmap) (s : SSAStore.t) (v : var),
+      Store.acc v (dessa_state m s) = SSAStore.acc (v, get_index v m) s.
+  Proof.
+    reflexivity.
+  Qed.
 
-   *)
+  Lemma ssa_dessaK :
+    forall (m : vmap) (s : Store.t) (x : var),
+      Store.acc x (dessa_state m (ssa_state m s)) = Store.acc x s.
+  Proof.
+    move=> m s x.
+    rewrite acc_dessa_state.
+    rewrite (acc_ssa_state_eq _ (eqxx (get_index x m))).
+    reflexivity.
+  Qed.
+
+  (* Definition dessa_typenv (m : vmap) (ste : SSATE.env) : TE.env := *)
+  (*   fun v => SSATE.vtyp (v, get_index v m) ste. *)
+
+  Definition dessa_typenv (m : vmap) (ste : SSATE.env) : TE.env :=
+    SSATE.fold (fun k v ste =>
+                  if sidx k == get_index (svar k) m then
+                    TE.add (svar k) v ste
+                  else ste
+               ) ste (TE.empty typ).
+
+  Lemma acc_dessa_typenv :
+    forall (m : vmap) (ste : SSATE.env) (v : var),
+      TE.vtyp v (dessa_typenv m ste) = SSATE.vtyp (v, get_index v m) ste.
+  Proof.
+  Admitted.
+
+  Lemma ssa_dessa_typenv_K :
+    forall (m : vmap) (te : TE.env) (x : var),
+      TE.vtyp x (dessa_typenv m (ssa_typenv m te)) = TE.vtyp x te.
+  Proof.
+    move=> m s x.
+    rewrite acc_dessa_typenv.
+    symmetry.
+    exact: ssa_typenv_preserve.
+  Qed.
+
+  (** Soundness and completeness *)
+
+  Theorem ssa_spec_sound (s : DSL.spec) :
+    SSA.valid_spec (ssa_spec s) -> DSL.valid_spec s.
+  Proof.
+    (* destruct s as [input pre pg post]. *)
+    (* rewrite /ssa_spec /=. *)
+    (* set t1 := ssa_typenv empty_vmap input. *)
+    (* have Heq_typ: (t1 = ssa_typenv empty_vmap input) by reflexivity. *)
+    (* set t2 := ssa_program empty_vmap pg. *)
+    (* have: (t2 = ssa_program empty_vmap pg) by reflexivity. *)
+    (* destruct t2 as [m ssa_p]. *)
+    (* move=> Hpg Hspec s1 s2 /= Hf Hepre Hep. *)
+    (* pose ss1 := ssa_state empty_vmap s1. *)
+    (* move: (ssa_state_equiv empty_vmap s1) => Heq1. *)
+    (* move: (ssa_typenv_equiv empty_vmap input) => Heq2. *)
+    (* symmetry in Hpg. *)
+    (* set tsucc := (DSL.program_succ_typenv pg input). *)
+    (* have Htsucc: (tsucc = (DSL.program_succ_typenv pg input)) by reflexivity. *)
+    (* move: (ssa_eval_program_succ Hpg Heq1 Heq2 Hep Htsucc) => [ss2 [ste2 [Hsep [H]]]] *)
+    (* move: (ssa_eval_bexp2 Heq1 Hf) => Hsf. *)
+    (* move: (Hspec ss1 ss2 Hsf Hesp) => /= Hsg. *)
+    (* exact: (ssa_eval_bexp1 Heq2 Hsg). *)
+  Admitted.
+
+  Theorem ssa_spec_complete (s : DSL.spec) :
+    DSL.valid_spec s -> SSA.valid_spec (ssa_spec s).
+  Proof.
+    (* destruct s as [f p g]. *)
+    (* rewrite /ssa_spec /=. *)
+    (* set t := ssa_program empty_vmap p. *)
+    (* have: (t = ssa_program empty_vmap p) by reflexivity. *)
+    (* destruct t as [m ssa_p]. *)
+    (* move=> Hp Hspec ss1 ss2 /= Hsf Hesp. *)
+    (* pose s1 := dessa_state empty_vmap ss1. *)
+    (* pose Heq1 := (dessa_state_equiv empty_vmap ss1). *)
+    (* move: (dessa_eval_program_succ (Logic.eq_sym Hp) Heq1 Hesp) => [s2 [Hep Heq2]]. *)
+    (* move: (ssa_eval_bexp1 Heq1 Hsf) => Hf. *)
+    (* move: (Hspec s1 s2 Hf Hep) => /= Hg. *)
+    (* exact: (ssa_eval_bexp2 Heq2 Hg). *)
+  Admitted.
 
   (** Well-formed SSA *)
 
@@ -1980,6 +2343,9 @@ Section MakeSSA.
 
   Definition ssa_vars_unchanged_instr vs i : bool :=
     SSAVS.for_all (ssa_unchanged_instr_var i) vs .
+
+  Definition ssa_var_unchanged_program v p : bool :=
+    all (ssa_var_unchanged_instr v) p.
 
   Definition ssa_unchanged_program_var p v : bool :=
     all (ssa_var_unchanged_instr v) p .
@@ -2022,9 +2388,9 @@ Section MakeSSA.
       |- SSAStore.acc ?x ?s1 = SSAStore.acc ?x ?s2 =>
       rewrite /ssa_var_unchanged_instr /SSA.lvs_instr in Hun;
       move : (SSA.VSLemmas.not_mem_singleton1 Hun) => {Hun};
-                                                     rewrite /SSAVS.SE.eq => /negP Hneq;
-                                                                            inversion_clear Heval;
-                                                                            neq_store_upd_acc
+                                                      rewrite /SSAVS.SE.eq => /negP Hneq;
+                                                                              inversion_clear Heval;
+                                                                              neq_store_upd_acc
     | Hun : is_true (ssa_var_unchanged_instr ?x ?i),
             Heval : SSA.eval_instr _ (?i) ?s1 ?s2
       |- SSAStore.acc ?x ?s1 = SSAStore.acc ?x ?s2 =>
@@ -2033,10 +2399,10 @@ Section MakeSSA.
       let Hneqv := fresh in
       rewrite /ssa_var_unchanged_instr /SSA.lvs_instr in Hun;
       move : (SSA.VSLemmas.not_mem_add1 Hun) => {Hun} [Hneqv Hun1];
-                                               move : (SSA.VSLemmas.not_mem_singleton1 Hun1) Hneqv => {Hun1};
-                                                                                                     rewrite /SSAVS.SE.eq => /negP Hneqw /negP Hneqv;
-                                                                                                                            inversion_clear Heval;
-                                                                                                                            neq_store_upd_acc
+                                                move : (SSA.VSLemmas.not_mem_singleton1 Hun1) Hneqv => {Hun1};
+                                                                                                       rewrite /SSAVS.SE.eq => /negP Hneqw /negP Hneqv;
+                                                                                                                               inversion_clear Heval;
+                                                                                                                               neq_store_upd_acc
     | Hun : is_true (ssa_var_unchanged_instr ?x ?i),
             Heval : SSA.eval_instr _ (?i) ?s1 ?s2
       |- SSAStore.acc ?x ?s1 = SSAStore.acc ?x ?s2 =>
@@ -2182,13 +2548,13 @@ Section MakeSSA.
     - elim: p Hmem => /=.
       + done.
       + move=> hd tl IH Hmem. case: (SSA.VSLemmas.mem_union1 Hmem) =>
-                             {Hmem} Hmem.
+                              {Hmem} Hmem.
         * rewrite /ssa_var_unchanged_instr Hmem. done.
         * rewrite (IH Hmem). by case: (ssa_var_unchanged_instr v hd).
     - move/negP/idP: Hmem => Hmem. elim: p Hmem => /=.
       + done.
       + move=> hd tl IH Hmem. move: (SSA.VSLemmas.not_mem_union1 Hmem) =>
-                             {Hmem} [Hmem1 Hmem2]. move: (IH Hmem2) => Hun.
+                              {Hmem} [Hmem1 Hmem2]. move: (IH Hmem2) => Hun.
         rewrite ssa_var_unchanged_instr_not_mem Hmem1 Hun. done.
   Qed.
 
@@ -2850,7 +3216,7 @@ Section MakeSSA.
         exact: Hssa1.
       + apply: (@ssa_unchanged_program_subset _ (SSA.vars_env te)).
         * exact: (ssa_unchanged_program_tl Huc).
-        * apply: SSA.well_formed_instr_subset_rvs.
+          apply SSA.well_formed_instr_subset_rvs.
           exact: (SSA.well_formed_program_cons1 Hwf).
   Qed.
 
@@ -2892,7 +3258,7 @@ Section MakeSSA.
     well_formed_ssa_program (SSA.sinputs s) (SSA.sprog s).
   Proof.
     move=> /andP [/andP [/andP [/andP [/andP Hpre Hwell] Hprog] Hvs] Hssa].
-    by rewrite /well_formed_ssa_program Hwell Hvs Hssa.
+      by rewrite /well_formed_ssa_program Hwell Hvs Hssa.
   Qed.
 
   Corollary well_formed_ssa_spec_pre_unchanged s :
@@ -2900,7 +3266,9 @@ Section MakeSSA.
     ssa_vars_unchanged_program (SSA.vars_bexp (SSA.spre s)) (SSA.sprog s).
   Proof.
     move=> /andP [/andP [/andP [/andP [/andP [Hwd Hwt] Hp] Hg] Hun] Hssa].
-    exact: (ssa_unchanged_program_subset Hun Hwd).
+    eapply ssa_unchanged_program_subset.
+    exact: Hun.
+    by rewrite -SSA.are_defined_subset.
   Qed.
 
   Corollary well_formed_ssa_spec_post_subset s :
@@ -2909,9 +3277,585 @@ Section MakeSSA.
                  (SSA.vars_env (SSA.program_succ_typenv (SSA.sprog s) (SSA.sinputs s))).
   Proof.
     move=> /andP [/andP [/andP [/andP [ /andP [Hwd Hwt] Hp] /andP [Hwd2 Hwt2]] Hun] Hssa].
-    exact: Hwd2.
+    by rewrite -SSA.are_defined_subset.
   Qed.
 
+  Ltac le_ssa_var_unchanged_instr :=
+    match goal with
+    | H : ssa_instr _ _ = (_, _) |- _ =>
+      case: H; move=> _ <-; le_ssa_var_unchanged_instr
+    | |- is_true (ssa_var_unchanged_instr (?v, ?iv) ?i) =>
+      rewrite /ssa_var_unchanged_instr /=; le_ssa_var_unchanged_instr
+    | H : is_true (?iv <=? get_index ?v ?m)
+      |- is_true (~~ SSAVS.mem (?v, ?iv) (SSAVS.singleton (ssa_var (upd_index ?x ?m) ?x))) =>
+      let Hmem := fresh in
+      let Heq := fresh in
+      let Hv := fresh in
+      let Hi := fresh in
+      apply/negP => /= Hmem;
+                   move: (SSA.VSLemmas.mem_singleton1 Hmem) => {Hmem} Heq;
+                                                              move/eqP: Heq => [Hv Hi];
+                                                                              rewrite Hv Hi in H;
+                                                                              exact: (get_upd_index_leF H)
+    | H : is_true (?iv <=? get_index ?v ?m)
+      |- is_true (~~ SSAVS.mem (?v, ?iv)
+                    (SSAVS.add
+                       (ssa_var (upd_index ?v1 (upd_index ?v2 ?m)) ?v1)
+                       (SSAVS.singleton (ssa_var (upd_index ?v2 ?m) ?v2)))) =>
+      let Hmem := fresh in
+      let Hv := fresh in
+      let Hi := fresh in
+      apply/negP => /= Hmem;
+                   move: (SSA.VSLemmas.mem_add1 Hmem); case => {Hmem} Hmem;
+                                                              [ move/eqP: Hmem => [Hv Hi]; rewrite Hv Hi in H;
+                                                                                 apply: (@get_upd_index_leF (upd_index v2 m) v1);
+                                                                                 apply: (Nleq_trans H); exact: get_upd_index_le
+                                                              |
+                                                              move: (SSA.VSLemmas.mem_singleton1 Hmem) => {Hmem} Hmem;
+                                                                                                         move/eqP: Hmem => [Hv Hi]; rewrite Hv Hi in H;
+                                                                                                                          exact: (@get_upd_index_leF m v2)
+                                                              ]
+    | |- _ => idtac
+    end.
+
+  Lemma ssa_instr_le_unchanged m1 m2 i si :
+    forall v iv,
+      iv <=? get_index v m1 ->
+      ssa_instr m1 i = (m2, si) ->
+      ssa_var_unchanged_instr (v, iv) si.
+  Proof.
+    elim: i m1 m2 si; intros; by le_ssa_var_unchanged_instr.
+  Qed.
+
+  Lemma ssa_program_le_unchanged m1 m2 p sp :
+    forall v i,
+      i <=? get_index v m1 ->
+      ssa_program m1 p = (m2, sp) ->
+      ssa_var_unchanged_program (v, i) sp.
+  Proof.
+    elim: p m1 m2 sp.
+    - move=> m1 m2 sp v i Hi /= [Hm Hp].
+        by rewrite -Hp.
+    - move=> hd tl IH m1 m2 sp v i Hle Hsp.
+      move: (ssa_program_cons Hsp) => {Hsp} [m3 [shd [stl [Hshd [Hstl Hsp]]]]].
+      rewrite Hsp => {Hsp sp} /=.
+      apply/andP; split.
+      + exact: (ssa_instr_le_unchanged Hle Hshd).
+      + move: (ssa_instr_index_le v Hshd) => Hle2.
+        move: (Nleq_trans Hle Hle2) => {Hle Hle2} Hle.
+        exact: (IH _ _ _ _ _ Hle Hstl).
+  Qed.
+
+  Ltac ssa_lv_hd_unchanged_tl :=
+    match goal with
+    | Hstl : ssa_program ?m3 ?tl = (?m2, ?stl),
+             H : ssa_instr ?m1 ?hd = (?m3, ?shd)
+      |- _ =>
+      move: Hstl; case: H => <- <- /= Hstl; ssa_lv_hd_unchanged_tl
+    | Hstl : ssa_program (upd_index ?v ?m1) ?tl = (?m2, ?stl)
+      |- is_true (ssa_vars_unchanged_program
+                    (SSAVS.singleton (ssa_var (upd_index ?v ?m1) ?v)) ?stl) =>
+      apply: ssa_unchanged_program_singleton2;
+      apply: (ssa_program_le_unchanged _ Hstl);
+      exact: Nleqnn
+    | Hstl : ssa_program (upd_index ?v1 (upd_index ?v2 ?m1)) ?tl = (?m2, ?stl)
+      |- is_true (ssa_vars_unchanged_program
+                    (SSAVS.add
+                       (ssa_var (upd_index ?v1 (upd_index ?v2 ?m1)) ?v1)
+                       (SSAVS.singleton
+                          (ssa_var (upd_index ?v2 ?m1) ?v2))) ?stl) =>
+      apply: ssa_unchanged_program_add2; split;
+      [ apply: (ssa_program_le_unchanged _ Hstl);
+        exact: Nleqnn
+      | apply ssa_unchanged_program_singleton2;
+        apply: (ssa_program_le_unchanged _ Hstl);
+        exact: get_upd_index_le ]
+    | |- _ => idtac
+    end.
+
+  Theorem ssa_program_single_assignment m1 m2 p sp :
+    ssa_program m1 p = (m2, sp) ->
+    ssa_single_assignment sp.
+  Proof.
+    elim: p m1 m2 sp.
+    - move=> m1 m2 sp [] _ <-.
+      done.
+    - move=> hd tl IH m1 m2 sp Hsp.
+      move: (ssa_program_cons Hsp) => {Hsp} [m3 [shd [stl [Hshd [Hstl ->]]]]].
+      apply/andP; split.
+      + case: hd Hshd; intros; by ssa_lv_hd_unchanged_tl.
+      + exact: (IH _ _ _ Hstl).
+  Qed.
+
+  Lemma ssa_vars_env_comm m te :
+    SSAVS.Equal (SSA.vars_env (ssa_typenv m te))
+                (ssa_vars m (DSL.vars_env te)).
+  Proof.
+    intro.
+    split.
+    - move=> Hin.
+      rewrite /ssa_vars.
+  Admitted.
+
+  Lemma ssa_instr_well_defined te m1 m2 i si :
+    DSL.well_defined_instr te i ->
+    ssa_instr m1 i = (m2, si) ->
+    SSA.well_defined_instr (ssa_typenv m1 te) si.
+  Proof.
+    rewrite /DSL.well_defined_instr /SSA.well_defined_instr.
+    rewrite /DSL.are_defined /SSA.are_defined.
+    case: i => /=; intros;
+                repeat (match goal with
+                        | H : (_, _) = (_, _) |- _ => case: H => _ <- /=
+                        | H : is_true (_ && _) |- _ =>
+                          let H1 := fresh in
+                          let H2 := fresh in
+                          move/andP: H => [H1 H2]
+                        | |- is_true (_ && _) => apply/andP; split
+                        | H : is_true (VS.subset (DSL.vars_atomic ?a) ?vs)
+                          |- is_true (SSAVS.subset
+                                       (SSA.vars_atomic (ssa_atomic ?m ?a))
+                                       (ssa_vars ?m ?vs)) =>
+                          rewrite ssa_vars_atomic_subset; assumption
+                        | H : is_true (?v1 != ?v2)
+                          |- is_true (ssa_var (upd_index ?v1 (upd_index ?v2 ?m)) ?v1 !=
+                                             ssa_var (upd_index ?v2 ?m) ?v2) =>
+                          exact: (pair_neq1 _ _ H)
+                        | H : is_true (VS.mem ?v ?vs) |-
+                          is_true (SSAVS.mem (ssa_var ?m ?v) (ssa_vars ?m ?vs)) =>
+                          rewrite ssa_vars_mem1; exact: H
+                        | |- is_true(true) => done end) .
+    - move: (VS.for_all_2 (DSL.are_defined_compat te) H) => {H} H.
+      rewrite (SSAVS.for_all_1 (SSA.are_defined_compat (ssa_typenv m1 te))).
+      + done.
+      + intros x Hin.
+        rewrite <- ssa_vars_atomic_comm in Hin.
+        Admitted.
+  (*   all: try by rewrite ssa_vars_env_comm -ssa_vars_atomic_comm ssa_vars_subset. *)
+  (*     by rewrite ssa_vars_env_comm -ssa_vars_bexp_comm ssa_vars_subset. *)
+  (* Qed. *)
 
 
+  Lemma ssa_instr_well_typed te m1 m2 i si :
+    DSL.well_typed_instr te i ->
+    ssa_instr m1 i = (m2, si) ->
+    SSA.well_typed_instr (ssa_typenv m1 te) si.
+  Proof.
+    case: i => /=; intros;
+                repeat (match goal with
+                        | H : (_, _) = (_, _) |- _ => case: H => _ <- /=
+                        | H : is_true (_ && _) |- _ =>
+                          let H1 := fresh in
+                          let H2 := fresh in
+                          move/andP: H => [H1 H2]
+                        | |- is_true (_ && _) => apply/andP; split
+                        | H : is_true (?v1 != ?v2)
+                          |- is_true (ssa_var (upd_index ?v1 (upd_index ?v2 ?m)) ?v1 !=
+                                             ssa_var (upd_index ?v2 ?m) ?v2) =>
+                          exact: (pair_neq1 _ _ H)
+                        | |- is_true(true) => done end) .
+    (* need some lemmas *)
+  Admitted.
+
+
+  Lemma ssa_instr_well_formed te m1 m2 i si :
+    DSL.well_formed_instr te i ->
+    ssa_instr m1 i = (m2, si) ->
+    SSA.well_formed_instr (ssa_typenv m1 te) si.
+  Proof.
+    move=> /andP [Hwd Hwt] Hsi.
+    rewrite /SSA.well_formed_instr.
+      by rewrite (ssa_instr_well_defined Hwd Hsi) (ssa_instr_well_typed Hwt Hsi).
+  Qed.
+
+  (* ite: input typenv, lte: ?? *)
+  Definition dclosed m (ite lte :TE.env) (ste: SSATE.env) : Prop :=
+    (* Indices of unused variables should not be updated. *)
+    (forall v, (~~ TE.mem v ite /\ ~~ TE.mem v lte) -> get_index v m = 0) /\
+    (* The index of a variable in lte should start from 1. *)
+    (forall v, TE.mem v lte -> 0 <? get_index v m) /\
+    (* ste contains all versions of ite and lte. *)
+    (forall v i, SSATE.mem (v, i) ste = (TE.mem v ite) && (i <=? get_index v m) || (TE.mem v lte) && (0 <? i <=? get_index v m)).
+
+  Lemma dclosed_lte_idx_gt0 m ite lte ste v :
+    dclosed m ite lte ste -> TE.mem v lte -> 0 <? get_index v m.
+  Proof.
+    move=> [_ [H _]]. exact: H.
+  Qed.
+
+  Lemma dclosed_not_mem m ite lte ste v :
+    dclosed m ite lte ste ->
+    ~~ TE.mem v ite /\ ~~ TE.mem v lte ->
+    get_index v m = 0.
+  Proof.
+    move=> [Hd _] Hmem.
+    exact: (Hd v Hmem).
+  Qed.
+
+  Lemma dclosed_mem1 m ite lte ste v i :
+    dclosed m ite lte ste ->
+    SSATE.mem (v, i) ste ->
+    (TE.mem v ite) /\ (i <=? get_index v m) \/
+                     (TE.mem v lte) /\ (0 <? i <=? get_index v m).
+  Proof.
+    move=> [_ [_ Hd]] Hmem.
+    rewrite Hd in Hmem.
+    case: (orP Hmem) => {Hmem} /andP H.
+    - left; assumption.
+    - right; assumption.
+  Qed.
+
+  Lemma dclosed_mem2 m ite lte ste (v i: VarOrder.T) :
+    dclosed m ite lte ste ->
+    TE.mem v ite -> i <=? get_index v m ->
+    SSATE.mem (v, i) ste.
+  Proof.
+    move=> [_ [_ Hd]] Hmem Hi.
+    rewrite Hd.
+    apply/orP; left; apply/andP; split; assumption.
+  Qed.
+
+  Lemma dclosed_mem3 m ite lte ste (v i: VarOrder.T) :
+    dclosed m ite lte ste ->
+    TE.mem v lte -> 0 <? i <=? get_index v m ->
+    SSATE.mem (v, i) ste.
+  Proof.
+    move=> [_ [_ Hd]] Hmem Hi.
+    rewrite Hd.
+    apply/orP; right; apply/andP; split; assumption.
+  Qed.
+
+  Lemma dclosed_mem4 m ite lte ste v :
+    dclosed m ite lte ste ->
+    TE.mem v lte -> 0 <? get_index v m.
+  Proof.
+    move=> [_ [Hd _]] Hmem.
+    exact: (Hd _ Hmem).
+  Qed.
+(*
+  Lemma dclosed_mem5 m ite lte ste (v i: VarOrder.T) :
+    dclosed m ite lte ste ->
+    0 <? i <=? get_index v m ->
+    SSATE.mem (v, i) ste.
+  Proof.
+  Admitted.
+  (*   move=> Hd Hi. *)
+  (*   case Hmem: (TE.mem v (TE_union ite lte)). *)
+  (*   - case: (VS.Lemmas.mem_union1 Hmem) => {Hmem} Hmem. *)
+  (*     + move/andP: Hi => [Hi1 Hi2]. *)
+  (*       exact: (dclosed_mem2 Hd Hmem Hi2). *)
+  (*     + exact: (dclosed_mem3 Hd Hmem Hi). *)
+  (*   - move/idP/negP: Hmem => Hmem. *)
+  (*     rewrite (dclosed_not_mem Hd Hmem) in Hi. *)
+  (*     move/andP: Hi => [Hi1 Hi2]. *)
+  (*     rewrite Nleqn0 in Hi2. *)
+  (*     rewrite (eqP Hi2) Nltnn in Hi1. *)
+  (*     discriminate. *)
+  (* Qed. *)
+
+  Lemma dclosed_mem6 m ivs lvs svs v :
+    dclosed m ivs lvs svs ->
+    VS.mem v (VS.union ivs lvs) ->
+    SSAVS.mem (ssa_var m v) svs.
+  Proof.
+    move=> Hd Hmv. set sv := ssa_var m v. have: sv = ssa_var m v by reflexivity.
+    destruct sv as [x i]. move=> [] -> ->. case: (VS.Lemmas.mem_union1 Hmv) => {Hmv} Hmv.
+    - apply: (dclosed_mem2 Hd Hmv). exact: N.leb_refl.
+    - apply: (dclosed_mem3 Hd Hmv). rewrite (dclosed_lvs_idx_gt0 Hd Hmv) N.leb_refl.
+      done.
+  Qed.
+
+  Lemma dclosed_empty vs :
+    dclosed empty_vmap vs VS.empty (ssa_vars empty_vmap vs).
+  Proof.
+    split; first by reflexivity.
+    split; first by discriminate.
+    move=> v i.
+    case Hmem: (VS.mem v vs && (i <=? get_index v empty_vmap)
+                || [&& VS.mem v VS.empty, 0 <? i & i <=? get_index v empty_vmap]).
+    - case: (orP Hmem) => {Hmem} /andP [Hmem Hidx].
+      + apply: (ssa_vars_mem3 Hmem).
+        rewrite get_index_empty Nleqn0 in Hidx *.
+        exact: (eqP Hidx).
+      + discriminate.
+    - apply/negP => H.
+      move/negP: Hmem; apply.
+      move: (ssa_vars_mem2 H) => [y [[Hy Hidy] Hmemy]].
+      apply/orP; left; apply/andP; split.
+      + rewrite Hy; exact: Hmemy.
+      + rewrite Hidy Hy; exact: Nleqnn.
+  Qed.
+
+  Lemma dclosed_subset m ivs lvs svs :
+    dclosed m ivs lvs svs ->
+    SSAVS.subset (ssa_vars m (VS.union ivs lvs)) svs.
+  Proof.
+    move=> [Hd1 [Hd2 Hd3]].
+    apply: SSAVS.subset_1 => x /SSAVS.Lemmas.memP Hmem.
+    apply/SSAVS.Lemmas.memP.
+    move: Hmem; rewrite ssa_vars_union => Hmem.
+    destruct x as [x i].
+    rewrite Hd3; apply/orP.
+    case: (SSAVS.Lemmas.mem_union1 Hmem) => {Hmem} Hmem.
+    - left.
+      move: (ssa_vars_mem2 Hmem) => [y [[Hxy Hidx] Hmemy]].
+      apply/andP; split.
+      + rewrite Hxy; exact: Hmemy.
+      + rewrite Hidx Hxy; exact: Nleqnn.
+    - right.
+      move: (ssa_vars_mem2 Hmem) => [y [[Hxy Hidx] Hmemy]].
+      apply/andP; split.
+      + rewrite Hxy; exact: Hmemy.
+      + move: (Hd2 _ Hmemy) => H.
+        rewrite Hxy Hidx; apply/andP; split.
+        * assumption.
+        * exact: Nleqnn.
+  Qed.
+
+  Ltac dclosed_instr_well_formed_tac :=
+    match goal with
+    | H : (_, _) = (_, _) |- _ =>
+      case: H => _ <- /=; dclosed_instr_well_formed_tac
+    | H : is_true (_ && _) |- _ =>
+      let H1 := fresh in
+      let H2 := fresh in
+      move/andP: H => [H1 H2]; dclosed_instr_well_formed_tac
+    | |- is_true (_ && _) => apply/andP; split; dclosed_instr_well_formed_tac
+    | Hs : is_true (VS.subset (DSL.vars_atomic ?a) (VS.union ?ivs ?lvs)),
+           Hd : dclosed ?m1 ?ivs ?lvs ?svs
+      |- is_true (SSAVS.subset
+                   (SSA.vars_atomic (ssa_atomic ?m1 ?a))
+                   ?svs) =>
+      apply: (SSA.VSLemmas.subset_trans (s2:=ssa_vars m1 (VS.union ivs lvs)));
+      [ rewrite ssa_vars_atomic_subset;
+        assumption
+      | exact: dclosed_subset ]
+    | H : is_true (?v1 != ?v2)
+      |- is_true (ssa_var (upd_index ?v1 (upd_index ?v2 ?m)) ?v1 !=
+                         ssa_var (upd_index ?v2 ?m) ?v2) =>
+      exact: (pair_neq1 _ _ H)
+    | H1 : dclosed ?m ?ivs ?lvs ?svs,
+           H2 : is_true (VS.mem ?v (VS.union ?ivs ?lvs)) |-
+      is_true (SSAVS.mem (ssa_var ?m ?v) ?svs) =>
+      exact: (dclosed_mem6 H1 H2)
+    | |- _ => idtac
+    end.
+
+  Lemma dclosed_instr_well_formed ivs lvs svs m1 m2 i si :
+    DSL.well_formed_instr (TE.union ivs lvs) i ->
+    ssa_instr m1 i = (m2, si) ->
+    dclosed m1 ivs lvs svs ->
+    SSA.well_formed_instr svs si.
+  Proof.
+    case: i => /=; intros; by dclosed_instr_well_formed_tac.
+  Qed.
+*)
 End MakeSSA.
+
+  (* TODO: Check if all variables in a program are not indexed. *)
+
+  (*
+  Definition unindexed_var (v : var) : bool :=
+    vidx v == 1.
+
+  Definition unindexed_vars vs := VS.for_all unindexed_var vs.
+
+  Definition unindexed_atomic  (a : atomic) : bool :=
+    match a with
+    | Avar v => unindexed_var v
+    | Aconst ty n => true
+    end.
+
+  Fixpoint unindexed_eexp (e: eexp) :=
+    match e with
+    | Evar v => unindexed_var v
+    | Econst c => true
+    | Eunop op e => unindexed_eexp e
+    | Ebinop op e1 e2 => unindexed_eexp e1 && unindexed_eexp e2
+    end.
+
+  Fixpoint unindexed_rexp (e: rexp) :=
+    match e with
+    | Rvar v => unindexed_var v
+    | Rconst w n => true
+    | Runop w op e => unindexed_rexp e
+    | Rbinop w op e1 e2 => unindexed_rexp e1 && unindexed_rexp e2
+    | Ruext w e i => unindexed_rexp e
+    | Rsext w e i => unindexed_rexp e
+    end.
+
+  Fixpoint unindexed_ebexp (e: ebexp) :=
+    match e with
+    | Etrue => true
+    | Eeq e1 e2 => unindexed_eexp e1 && unindexed_eexp e2
+    | Eeqmod e1 e2 p => unindexed_eexp e1 && unindexed_eexp e2 && unindexed_eexp p
+    | Eand e1 e2 => unindexed_ebexp e1 && unindexed_ebexp e2
+    end.
+
+  Fixpoint unindexed_rbexp (e: rbexp) :=
+    match e with
+    | Rtrue => true
+    | Req w e1 e2 => unindexed_rexp e1 && unindexed_rexp e2
+    | Rcmp w op e1 e2 => unindexed_rexp e1 && unindexed_rexp e2
+    | Rneg e =>  unindexed_rbexp e
+    | Rand e1 e2 => unindexed_rbexp e1 && unindexed_rbexp e2
+    | Ror e1 e2 => unindexed_rbexp e1 && unindexed_rbexp e2
+    end.
+
+  Definition unindexed_bexp e := unindexed_ebexp (eqn_bexp e) && unindexed_rbexp (rng_bexp e).
+
+  Definition unindexed_instr (i: instr) : bool :=
+    match i with
+    | Imov v a
+    | Ishl v a _ =>
+      let v := unindexed_var v in
+      let a := unindexed_atomic a in
+      v && a
+    | Icshl vh vl a1 a2 _ =>
+      let vh := unindexed_var vh in
+      let vl := unindexed_var vl in
+      let a1 := unindexed_atomic a1 in
+      let a2 := unindexed_atomic a2 in
+      vh && vl && a1 && a2
+    | Inondet v =>
+      let v := unindexed_var v in v
+    | Icmov v c a1 a2 =>
+      let v := unindexed_var v in
+      let c := unindexed_atomic c in
+      let a1 := unindexed_atomic a1 in
+      let a2 := unindexed_atomic a2 in
+      v && c && a1 && a2
+    | Inop => true
+    | Inot v a =>
+      let v := unindexed_var v in
+      let a := unindexed_atomic a in
+      v && a
+    | Iadd v a1 a2 =>
+      let v := unindexed_var v in
+      let a1 := unindexed_atomic a1 in
+      let a2 := unindexed_atomic a2 in
+      v && a1 && a2
+    | Iadds c v a1 a2
+    | Iaddr c v a1 a2 =>
+      let c := unindexed_var c in
+      let v := unindexed_var v in
+      let a1 := unindexed_atomic a1 in
+      let a2 := unindexed_atomic a2 in
+      c && v && a1 && a2
+    | Iadc v a1 a2 y =>
+      let v := unindexed_var v in
+      let a1 := unindexed_atomic a1 in
+      let a2 := unindexed_atomic a2 in
+      let y := unindexed_atomic y in
+      v && a1 && a2 && y
+    | Iadcs c v a1 a2 y
+    | Iadcr c v a1 a2 y =>
+      let c := unindexed_var c in
+      let v := unindexed_var v in
+      let a1 := unindexed_atomic a1 in
+      let a2 := unindexed_atomic a2 in
+      let y := unindexed_atomic y in
+      c && v && a1 && a2 && y
+    | Isub v a1 a2 =>
+      let v := unindexed_var v in
+      let a1 := unindexed_atomic a1 in
+      let a2 := unindexed_atomic a2 in
+      v && a1 && a2
+    | Isubc c v a1 a2
+    | Isubb c v a1 a2
+    | Isubr c v a1 a2 =>
+      let c := unindexed_var c in
+      let v := unindexed_var v in
+      let a1 := unindexed_atomic a1 in
+      let a2 := unindexed_atomic a2 in
+      c && v && a1 && a2
+    | Isbc v a1 a2 y =>
+      let v := unindexed_var v in
+      let a1 := unindexed_atomic a1 in
+      let a2 := unindexed_atomic a2 in
+      let y := unindexed_atomic y in
+      v && a1 && a2 && y
+    | Isbcs c v a1 a2 y
+    | Isbcr c v a1 a2 y =>
+      let c := unindexed_var c in
+      let v := unindexed_var v in
+      let a1 := unindexed_atomic a1 in
+      let a2 := unindexed_atomic a2 in
+      let y := unindexed_atomic y in
+      c && v && a1 && a2 && y
+    | Isbb v a1 a2 y =>
+      let v := unindexed_var v in
+      let a1 := unindexed_atomic a1 in
+      let a2 := unindexed_atomic a2 in
+      let y := unindexed_atomic y in
+      v && a1 && a2 && y
+    | Isbbs c v a1 a2 y
+    | Isbbr c v a1 a2 y =>
+      let c := unindexed_var c in
+      let v := unindexed_var v in
+      let a1 := unindexed_atomic a1 in
+      let a2 := unindexed_atomic a2 in
+      let y := unindexed_atomic y in
+      c && v && a1 && a2 && y
+    | Imul v a1 a2 =>
+      let v := unindexed_var v in
+      let a1 := unindexed_atomic a1 in
+      let a2 := unindexed_atomic a2 in
+      v && a1 && a2
+    | Imuls c v a1 a2
+    | Imulr c v a1 a2 =>
+      let c := unindexed_var c in
+      let v := unindexed_var v in
+      let a1 := unindexed_atomic a1 in
+      let a2 := unindexed_atomic a2 in
+      c && v && a1 && a2
+    | Imull vh vl a1 a2 =>
+      let vh := unindexed_var vh in
+      let vl := unindexed_var vl in
+      let a1 := unindexed_atomic a1 in
+      let a2 := unindexed_atomic a2 in
+      vh && vl && a1 && a2
+    | Imulj v a1 a2 =>
+      let v := unindexed_var v in
+      let a1 := unindexed_atomic a1 in
+      let a2 := unindexed_atomic a2 in
+      v && a1 && a2
+    | Isplit vh vl a n =>
+      let vh := unindexed_var vh in
+      let vl := unindexed_var vl in
+      let a := unindexed_atomic a in
+      vh && vl && a
+    | Iand v a1 a2
+    | Ior v a1 a2
+    | Ixor v a1 a2 =>
+      let v := unindexed_var v in
+      let a1 := unindexed_atomic a1 in
+      let a2 := unindexed_atomic a2 in
+      v && a1 && a2
+    | Icast v a
+    | Ivpc v a =>
+      let v := unindexed_var v in
+      let a := unindexed_atomic a in
+      v && a
+    | Ijoin v ah al =>
+      let v := unindexed_var v in
+      let ah := unindexed_atomic ah in
+      let al := unindexed_atomic al in
+      v && ah && al
+    | Iassert e => unindexed_bexp e
+    | Iassume e => unindexed_bexp e
+    | Iecut e pwss => unindexed_ebexp e
+    | Ircut e pwss => unindexed_rbexp e
+    | Ighost vs e => unindexed_vars vs && unindexed_bexp e
+    end.
+
+  Fixpoint unindexed_program (p : program) : bool :=
+    match p with
+    | [::] => true
+    | hd::tl =>
+      let unidx_instr := unindexed_instr hd in
+      let unidx_tl := unindexed_program tl in
+      unidx_instr && unidx_tl
+    end.
+
+   *)
